pancake/panLangScript.sml
@@ -17,9 +17,6 @@ Type varname = ``:mlstring``
 
 Type funname = ``:mlstring``
 
-Type time = ``:num``
-
-
 val _ = Datatype `
   exp = Const ('a word)
       | Var varname
@@ -45,7 +42,8 @@ val _ = Datatype `
        | Break
        | Continue
        | Call ret ('a exp) (('a exp) list)
-       | ExtCall funname varname (('a exp) list)
+       (*  | ExtCall funname varname (('a exp) list) *)
+       | ExtCall funname varname varname varname varname (* FFI name, conf_ptr, conf_len, array_ptr, array_len*)
        | Raise ('a exp)
        | Return ('a exp)
        | Tick
